Nerodia/Data/Codec/Errors.lean
@@ -26,17 +26,17 @@ The Lean names of these Python identifiers follow Lean naming conventions
 -/
 
 /-- Raise {lit}`UnicodeError` (or a subclass). -/
-public abbrev strict : CodecErrors := ⟨"strict"⟩
+@[inline] public def strict : CodecErrors := ⟨"strict"⟩
 
 /-- Ignore the malformed data and continue without further notice. -/
-public abbrev ignore : CodecErrors := ⟨"ignore"⟩
+@[inline] public def ignore : CodecErrors := ⟨"ignore"⟩
 
 /--
 Replace unspported characters with a replacement marker. On encoding,
 use `?` (the ASCII character). On decoding, use `�` (U+FFFD, the official
 Unicode replacement character).
 -/
-public abbrev replace : CodecErrors := ⟨"replace"⟩
+@[inline] public def replace : CodecErrors := ⟨"replace"⟩
 
 /--
 Replace unspported characters with backslashed escape sequences.
@@ -44,7 +44,7 @@ On encoding,  use hexadecimal form of Unicode code point with formats
 {lit}`\xhh`, {lit}`\uxxxx`, {lit}`\Uxxxxxxxx`. On decoding, use hexadecimal
 form of byte value with format {lit}`\xhh`.
 -/
-public abbrev backslashReplace : CodecErrors := ⟨"backslashreplace"⟩
+@[inline] public def backslashReplace : CodecErrors := ⟨"backslashreplace"⟩
 
 /--
 On decoding, replace surrogates with their individual surrogate escape
@@ -52,25 +52,25 @@ code ranging from {lit}`U+DC80` to {lit}`U+DCFF`. This code will then be turned
 back into the surrogate when the {name}`surrogateEscape` error handler is
 used when encoding the data.
 -/
-public abbrev surrogateEscape : CodecErrors := ⟨"surrogateescape"⟩
+@[inline] public def surrogateEscape : CodecErrors := ⟨"surrogateescape"⟩
 
 /--
 For Unicode codecs, allow encoding and decoding a surrogate code point
 ({lit}`U+D800` - {lit}`U+DFFF`) as normal code point. Otherwise, these codecs
 treat the presence of a lone surrogate as an error.
 -/
-public abbrev surrogatePass : CodecErrors := ⟨"surrogatepass"⟩
+@[inline] public def surrogatePass : CodecErrors := ⟨"surrogatepass"⟩
 
 /--
 When encoding text, replace unspported characters with XML/HTML numeric
 character reference, which is a decimal form of Unicode code point with
 format `&#num;`.
 -/
-public abbrev xmlCharRefReplace : CodecErrors := ⟨"xmlcharrefreplace"⟩
+@[inline] public def xmlCharRefReplace : CodecErrors := ⟨"xmlcharrefreplace"⟩
 
 /--
 When encoding text, replace unspported characters with {lit}`\N{...}`
 escape sequences. What appears in the braces is the {lit}`Name` property
 from the Unicode Character Database.
 -/
-public abbrev nameReplace : CodecErrors := ⟨"namereplace"⟩
+@[inline] public def nameReplace : CodecErrors := ⟨"namereplace"⟩
